ulib/experimental/Steel.SpinLock.fst
@@ -15,7 +15,7 @@ let locked = true
 let lockinv (p:hprop) (r:ref bool) : hprop =
   h_exists (fun b -> pts_to r full_perm (Ghost.hide b) `star` (if b then emp else p))
 
-let lock (p:hprop u#1) = (r:ref bool) & inv (lockinv p r)
+let lock (p:hprop u#1) = (r:ref bool) & ival (lockinv p r)
 
 val intro_lockinv_available (#uses:Set.set lock_addr) (p:hprop) (r:ref bool)
   : SteelAtomic unit uses true (pts_to r full_perm available `star` p) (fun _ -> lockinv p r)
@@ -37,19 +37,19 @@ let intro_lockinv_locked #uses p r =
     (fun b -> pts_to r full_perm (Ghost.hide (U.downgrade_val b)) `star`
       (if (U.downgrade_val b) then emp else p))
 
-val new_inv (p:hprop) : SteelT (inv p) p (fun _ -> emp)
+val new_inv (p:hprop) : SteelT (ival p) p (fun _ -> emp)
 let new_inv p = lift_atomic_to_steelT (fun _ -> Steel.Effect.Atomic.new_inv p)
 
 #set-options "--fuel 0 --ifuel 0"
 
 let new_lock (p:hprop)
   : SteelT (lock p) p (fun _ -> emp) =
-  h_admit p (fun _ -> emp `star` p); // How to prove that ?
+  Steel.SteelT.Basics.h_intro_emp_l p;
   let r:ref bool =
     frame (fun _ -> alloc available) p
   in
   lift_atomic_to_steelT (fun _ -> intro_lockinv_available p r);
-  let i:inv (lockinv p r) = new_inv (lockinv p r) in
+  let i:ival (lockinv p r) = new_inv (lockinv p r) in
   let l:lock p = (| r, i |) in
   l
 
@@ -74,7 +74,7 @@ let cas_frame #t #uses r v v_old v_new frame =
     return_atomic x
   )
 
-val acquire_core (#p:hprop) (#u:Set.set lock_addr) (r:ref bool) (i:inv (lockinv p r))
+val acquire_core (#p:hprop) (#u:Set.set lock_addr) (r:ref bool) (i:ival (lockinv p r))
   : SteelAtomic bool u false
     (lockinv p r `star` emp)
     (fun b -> lockinv p r `star` (if b then p else emp))
@@ -95,7 +95,7 @@ let acquire_core #p #u r i =
 let acquire' (#p:hprop) (l:lock p)
   : SteelAtomic bool Set.empty false emp (fun b -> if b then p else emp)
   = let r:ref bool = dfst l in
-    let i: inv (lockinv p r) = dsnd l in
+    let i: ival (lockinv p r) = dsnd l in
     let b = with_invariant_frame i (fun _ -> acquire_core r i) in
     return_atomic #_ #_ #_ b
 
@@ -103,7 +103,7 @@ let rec acquire #p l =
   let b = lift_atomic_to_steelT (fun _ -> acquire' l) in
   cond b (fun b -> if b then p else emp) (fun _ _ -> p) noop (fun _ -> acquire l)
 
-val release_core (#p:hprop) (#u:Set.set lock_addr) (r:ref bool) (i:inv (lockinv p r))
+val release_core (#p:hprop) (#u:Set.set lock_addr) (r:ref bool) (i:ival (lockinv p r))
   : SteelAtomic bool u false
     (lockinv p r `star` p)
     (fun b -> lockinv p r `star` (if b then emp else p))
@@ -125,7 +125,7 @@ let release_core #p #u r i =
 
 let release #p l =
   let r:ref bool = dfst l in
-  let i: inv (lockinv p r) = dsnd l in
+  let i: ival (lockinv p r) = dsnd l in
   let b = lift_atomic_to_steelT (fun _ -> with_invariant_frame i
     (fun _ -> release_core r i))
   in
